src/RTL.v
@@ -1,5 +1,4 @@
 Require Import Common. 
-Require Import DList. 
 Require Import Core. 
 
      
@@ -13,32 +12,580 @@ Section t.
   Inductive bind (t : type) : Type := 
   | bind_expr :  expr R t ->  bind t
   | bind_reg_read : var Phi (Treg t) -> bind t
-  | bind_regfile_read : forall n, var Phi (Tregfile n t) -> forall p, R (Tlift (W p)) -> bind t. 
-  
-  Inductive effect  : Type :=
-  | effect_guard : forall (guard : expr R Bool), list (effect) -> effect 
-  | effect_reg_write : forall t, var Phi (Treg t) -> R t -> effect
-  | effect_regfile_write : forall n t, var Phi (Tregfile n t) -> forall p, R (Tlift (W p)) -> R t -> effect. 
-  
+  | bind_regfile_read : forall n, var Phi (Tregfile n t) -> R (Tlift (Tfin n)) -> bind t. 
+    
   Inductive telescope (A : Type): Type :=
   | telescope_end : A -> telescope A
   | telescope_bind : forall arg, bind arg -> (R arg -> telescope A) -> telescope A. 
+    
+  (* nested effects *)
+  Inductive neffect  : Type :=
+  | neffect_guard : forall (guard : expr R Bool), list (neffect) -> neffect 
+  | neffect_reg_write : forall t, var Phi (Treg t) -> R t -> neffect
+  | neffect_regfile_write : forall n t, var Phi (Tregfile n t) -> R (Tlift (Tfin n)) -> R t -> neffect. 
+
+  Definition nblock t := telescope (R t * expr R Bool * list neffect)%type. 
   
-  Definition preblock t := telescope (R t * expr R Bool * list effect)%type. 
-  Definition block := telescope (list effect). 
-  
-  Fixpoint compose {t B} 
-                   (tA : preblock t)
-                   (f : R t -> expr R Bool -> list effect -> telescope B) :
-    telescope B :=
+  Fixpoint compose {A B}
+                   (tA : telescope  A)
+                   (f : A -> telescope  B) :
+    telescope  B :=
     match tA with
-      | telescope_end ((r,g),e) => f r g e
-      | telescope_bind arg b cont => telescope_bind _ arg b (fun x => compose (cont x) f) 
-    end. 
-  
+      | telescope_end e => f e
+      | telescope_bind arg b cont => telescope_bind _  arg b (fun x => compose (cont x) f)
+    end.
+
+  Definition compose_block {t B} 
+                           (tA : nblock t)
+                           (f : R t -> expr R Bool -> list neffect -> telescope B) :
+    telescope B :=
+    compose tA (fun x => match x with ((r,g),e) => f r g e end). 
+  Hint Unfold compose_block. 
   Notation "x <- e1 ; e2" := (telescope_bind _ _ e1 (fun x => e2)) (right associativity, at level 80, e1 at next level).  
   Notation " & e " := (telescope_end _ e) (at level 71). 
-  Notation "[< r , g , e >] :- t1 ; t2 " := (compose t1 (fun r g e => t2)) (right associativity, at level 80, t1 at next level). 
+  Notation "[< r , g , e >] :- t1 ; t2 " := (compose_block t1 (fun r g e => t2)) (right associativity, at level 80, t1 at next level). 
+  
+  Arguments neffect_guard guard%expr neffects%list. 
+  
+  (** * Compilation *)
+  (** This 'smart constructor' reduces the size of the guard, by using
+  the fact that [true] is a neutral element for [&&] *)
+  
+  Definition andb (a b : expr R Bool): expr R Bool :=
+    match a, b with 
+      | Econstant Tbool x, o 
+      | o, Econstant Tbool x => if x then o else (#b false)%expr
+      | _, _ => (a && b)%expr
+    end. 
+  
+  (**  The compilation function itself *)
+  Variable varunit : R Unit. 
+  
+  Definition convert  l : DList.T (expr R) l -> Tuple.of_list (expr R) l := 
+    DList.to_tuple (fun t X => X). 
+
+  Fixpoint map T F F' (G : forall t, F t -> F' t) (l : list T) : 
+    Tuple.of_list F l -> Tuple.of_list F' l:=
+    match l with 
+      | nil => fun x => x
+      | cons t q => fun x => (G t (fst x), map T F F' G q (snd x))
+    end. 
+
+  Arguments map {T F F'} G l _. 
+  (*  fst (DList.T_fold' eval_expr [t] exprs) =
+   eval_expr t
+     (fst
+        (DList.T_fold' (fun (t0 : type) (X : expr eval_type t0) => X) [t] exprs))
+
+*)
+  
+  Definition compile  t (a : action Phi R t) : telescope (R t * expr R Bool * list neffect).  
+  refine (
+      let f := fix compile t (a : action Phi R t) : telescope (R t * expr R Bool * list neffect):= 
+          match a with 
+            | Return t exp =>  
+                x <- (bind_expr _ exp); 
+                & (x, #b true, nil)
+            | Bind t u A F => 
+                [< rA, gA, eA >] :- compile _ A;
+                [< rB, gB, eB >] :- compile _ (F rA); 
+                & (rB, andb gA gB, List.app eA eB)             
+            | Assert exp => 
+                x <- (bind_expr _ exp); 
+                & (varunit, !x, nil)%expr
+            | Primitive args res p exprs => _
+            (* | Try A =>  *)
+            (*     [< rA, gA, eA >] :- compile _ A; *)
+            (*     let e := neffect_guard gA eA in *)
+            (*       & (varunit, #b true, [e])%list *)
+            (*     (* & (varunit, gA, eA) *) *)
+            | OrElse t A A' => 
+                [< rA, gA, eA >] :- compile _ A;
+                [< rA', gA', eA' >] :- compile _ A';
+                let e := neffect_guard gA eA in 
+                let e' := neffect_guard ((~ gA) &&  gA')%expr eA' in 
+                  r <- (bind_expr _ (Emux _ _ gA (!rA) (!rA'))%expr); 
+                  & ( r , (gA || gA')%expr , [e;e'])%list
+          end in f t a).
+  (* primitive *)
+  revert exprs. 
+  refine (match p with
+            | register_read t v => _
+            | register_write t v => _
+            | regfile_read n t v  => _
+            | regfile_write n t v  => _
+          end); clear p; intros exprs. 
+  (* register read *)
+  refine (x <- (bind_reg_read _ v); &(x, #b true, nil)). 
+  (* register write *)
+  refine ( let env := convert _ exprs in 
+             let w := fst env in 
+               x <- bind_expr _ w; 
+           let e := ([neffect_reg_write _ v x])%list  in 
+             &( varunit, #b true, e)
+         ). 
+  (* register file read *)
+  refine ( let env := convert _ exprs in 
+             let adr := fst env in 
+               adr <- bind_expr _ adr; 
+           x <- bind_regfile_read _ _ v adr; 
+           &( x, #b true, nil)
+         ). 
+  (* register file write *)
+  refine ( let env := convert _ exprs in 
+             match env with 
+               | (adr, (w, _)) => 
+                   adr <- bind_expr _ adr; 
+                   w <- bind_expr _ w;
+                   let e :=  ([neffect_regfile_write _ _ v  adr w])%list in                      
+                     &( varunit, #b true, e)                      
+             end
+         ). 
+    (* or else *)
+  
+  Defined. 
+  
+  Inductive effect  : sync -> Type :=
+  | effect_reg_write : forall t,  R t -> R Bool -> effect (Treg t)
+  | effect_regfile_write : forall n t,  R t -> R (Tlift (Tfin n)) -> R Bool -> 
+                                                effect (Tregfile n t). 
+  
+  Definition effects := Tuple.of_list (option ∘ effect) Phi. 
+  Definition init_effects : effects. 
+  apply Tuple.init. intros.  apply None.     
+  Defined. 
+
+  Definition block t := telescope (R t * expr R Bool *  effects). 
+  
+  
+  Notation "e :-- t1 ; t2 " := (compose t1 (fun e => t2)) (right associativity, at level 80, e1 at next level).
+  Arguments Tuple.set {T F l t} _ _ _.  
+
+  Definition nblock_to_block {t} (B : nblock t) : block t. 
+  unfold block, nblock in *. 
+  
+
+  Definition update_Treg t (v : var Phi (Treg t)) (guard : R Bool) (val : R t) (acc : effects) : telescope effects. 
+  refine (match  Tuple.get _  _ v acc
+             with 
+               | Some old => _
+               | None =>       
+                   we <- bind_expr _  (!guard)%expr ; 
+                   w <- bind_expr _  (!val )%expr ; 
+                   & (Tuple.set v (Some (effect_reg_write _ w we)) acc )
+          end). 
+  refine (match old in effect s return match s with 
+                                   | Treg t =>  var Phi s -> R t -> telescope effects 
+                                   | _ => ID
+                               end
+  with
+    | effect_reg_write t' val' guard' => 
+        fun v val => 
+          we <- bind_expr  _ (!guard' || !guard)%expr ;
+          w <- bind_expr  _ (Emux _ _ (!guard') (!val') (!val) )%expr ;
+          & (Tuple.set v (Some (effect_reg_write  _ w we)) acc)
+    | _ => @id
+  end v val). 
+  Defined. 
+
+  Definition update_Tregfile n t (v : var Phi (Tregfile n t)) (guard : R Bool) (adr : R (Tlift (Tfin n)) ) (val : R t) (acc : effects) : telescope effects. 
+  
+  refine (match Tuple.get _ _ v acc with 
+              | Some old => _
+              | None =>       
+                  we <- bind_expr _  (!guard)%expr; 
+                  wadr <- bind_expr _  ((!adr)); 
+                  wdata <- bind_expr _ ((!val)); 
+                  & (Tuple.set v (Some (effect_regfile_write _ _ wdata wadr we)) acc)
+          end%expr
+         )%expr. 
+  
+  inversion old. subst.   
+  refine 
+    (
+      we <- bind_expr  _ (!X1 || !guard)%expr; 
+      wadr <- bind_expr _ (Emux _ _ (!X1) (!X0) (!adr)); 
+      wdata <- bind_expr _ (Emux _ _ (!X1) (!X) (!val)); 
+      & (Tuple.set v (Some (effect_regfile_write _ _ wdata wadr we)) acc)
+    )%expr. 
+  Defined. 
+
+  Fixpoint compile_neffect (G : expr R Bool) (E : neffect) (B : effects) : telescope effects :=
+    match E with               
+      | neffect_guard guard L => 
+                    let compile_neffects := fix compile_neffects G l U :=
+                        match l with 
+                          | nil =>  & U
+                          | cons t q => 
+                              compose (compile_neffect G t U)
+                                      (compile_neffects G q)
+                        end in 
+                      compile_neffects (G && guard)%expr L B
+      | neffect_reg_write t v val => 
+          G <- bind_expr _  G;
+          update_Treg t v G val B
+      | neffect_regfile_write n t v adr val => 
+          G <- bind_expr _  G;
+          update_Tregfile n t v G adr val B
+    end.  
+
+    
+  Fixpoint compile_neffects (G : expr R Bool)(l : list neffect)  (T : effects) :
+    telescope effects :=
+    match l with 
+      | nil =>  & T
+      | cons t q => 
+          compose (compile_neffect G  t T)
+                  (compile_neffects G q)
+    end. 
+
+ 
+  refine (compose_block B (fun res guard neffects => 
+                             compose (compile_neffects (#b true ) neffects (init_effects))
+                             (fun effects => &(res, guard, effects)))). 
+  Defined. 
+
+
+End defs. 
+  
+  (** * Semantics *)
+  Section sem. 
+    Variable st : eval_state Phi. 
+    Definition eval_bind t (b : bind eval_type t) : (eval_type t).
+    refine (match b with
+              | bind_expr x =>  (eval_expr _ x)
+              | bind_reg_read v => (Tuple.get _ _ v st)
+              | bind_regfile_read n v adr => 
+                  let rf := Tuple.get Phi (Tregfile n t) v st in
+                    Regfile.get rf (adr)                
+            end
+           ). 
+    Defined. 
+    
+                                                                
+    Fixpoint eval_neffect (e :neffect eval_type) (Delta : updates) : updates :=    
+      match e with 
+        | neffect_guard g l' => 
+            let fix eval_neffects l Delta := 
+                match l with 
+                  | nil => Delta
+                  | cons e q =>  
+                      let Delta := eval_neffect e Delta in 
+                        eval_neffects q Delta
+                end in     
+              match eval_expr _ g with 
+                | true => 
+                    eval_neffects l' Delta
+                | false => Delta
+            end
+      | neffect_reg_write t v w =>                                               
+          Core.Diff.add Phi Delta (Treg t) v w 
+      | neffect_regfile_write  n t v adr w  =>  
+          let rf := Tuple.get Phi (Tregfile n t) v st in                          
+            let rf := Regfile.set rf adr  w in 
+              Core.Diff.add Phi Delta (Tregfile n t) v rf            
+    end. 
+  
+    Fixpoint eval_neffects ( l : list (neffect eval_type)) Delta : updates :=
+      match l with 
+        | nil =>  Delta
+        | cons e q => (* do Delta <- eval_neffect e Delta;  *)
+            let Delta :=  (eval_neffect e Delta) in 
+            eval_neffects q Delta
+      end. 
+  
+    Lemma fold_eval_neffects :
+      (fix eval_neffects l Delta := 
+       match l with 
+                | nil =>  Delta
+                | cons e q => 
+                    let Delta := (eval_neffect e Delta) in 
+                      (* do Delta <- eval_neffect e Delta;  *)
+                      eval_neffects q Delta
+       end)= eval_neffects .
+    Proof. 
+      unfold eval_neffects. reflexivity.
+    Qed. 
+    
+    Fixpoint eval_nblock t  (T : nblock  eval_type t) :
+      updates -> option (eval_type t * updates) := 
+      match T with
+        | telescope_bind arg bind cont => 
+            fun Delta => 
+              let res := eval_bind _ bind in
+              eval_nblock _ (cont res) Delta
+        | telescope_end (p, g, e) => fun Delta =>
+                                      let g := eval_expr _ g  in             
+                                      if g then                                         
+                                        Some (p, eval_neffects e Delta)
+                                      else None
+    end. 
+
+    Definition eval_effect (e : effects eval_type) (Delta : updates) : updates.  
+    unfold effects in e. 
+    
+    refine (Tuple.map3 _ Phi e st  Delta).
+    refine (fun a eff => 
+              match eff with 
+                  | Some eff =>  
+                      match eff in effect _ s return eval_sync s -> (option ∘ eval_sync) s -> (option ∘ eval_sync) s  with 
+                        |  effect_reg_write t val we =>  fun _ old => 
+                             match old with 
+                               | Some _ => old
+                               | None => if we then Some val else None
+                             end
+                        |  effect_regfile_write n t val adr we => fun rf old =>
+                             match old with 
+                               | Some _ => old 
+                               | None => 
+                                   if we then 
+                                     let rf := Regfile.set rf adr val in 
+                                       Some rf
+                                   else 
+                                     None                                       
+                             end
+                      end
+                  | None => fun _ old => old
+              end). 
+    Defined. 
+
+    Fixpoint eval_block t  (T : block eval_type t) :
+      updates -> option (eval_type t * updates) := 
+      match T with
+        | telescope_bind arg bind cont => 
+            fun Delta => 
+              let res := eval_bind _ bind in
+              eval_block _ (cont res) Delta
+        | telescope_end (p, g, e) => fun Delta =>
+                                      let g := eval_expr _ g  in             
+                                      if g then                                         
+                                        Some (p, eval_effect e Delta)
+                                      else None
+    end. 
+  
+     
+  End sem. 
+
+
+  (* Notation "x <-- e1 ; e2" := (telescope_bind  _ _ _ e1 (fun x => e2)) (right associativity, at level 80, e1 at next level).   *)
+  (* Notation " & e " := (telescope_end  _ _ e) (at level 71).  *)
+  (* Notation "[< r , g , e >] :- t1 ; t2 " := (compose  _ t1 (fun r g e => t2)) (right associativity, at level 80, t1 at next level).  *)
+  
+  Section correctness. 
+  
+    
+    
+    Notation C := (compile eval_type tt). 
+    Lemma eval_andb_true x y : (eval_expr Bool (andb eval_type x y)) = (eval_expr Bool x && eval_expr Bool y)%bool.
+    Proof. 
+      Require Import Equality Bool. 
+      
+      dependent destruction x; dependent destruction y; simpl;
+      repeat match goal with 
+                 c : constant0 B |- _ => destruct c
+               | x : eval_type Bool |- _ => destruct x
+               | _ => idtac
+             end; rewrite ?andb_true_r, ?andb_true_l, ?andb_false_l , ?andb_false_r ; reflexivity.  
+    Qed. 
+
+    Lemma eval_neffects_append  st e f (Delta : updates) : 
+      eval_neffects st (e ++ f) Delta = 
+                   eval_neffects st f (eval_neffects st e Delta).              
+    Proof. 
+      revert Delta. 
+      induction e. 
+      + reflexivity. 
+      + intros Delta.
+        
+        simpl. rewrite IHe. reflexivity.  
+
+    Qed. 
+
+    Variable st : eval_state Phi. 
+
+    Notation "B / Delta " := (eval_nblock st _ B Delta). 
+    Theorem CPS_compile_correct t (a : action Phi eval_type t)  Delta:
+      eval_nblock st _ (C t a ) Delta =  (Core.Sem.eval_action a st Delta).
+    Proof. 
+      revert Delta. 
+      induction a. 
+      - intros.  reflexivity. 
+      - intros Delta. simpl. unfold  Sem.Dyn.Bind. rewrite <- IHa.
+        transitivity (do ed <- (C t a) / Delta ; 
+                      let (e,d) := ed in 
+                      eval_nblock st u (C u (f e)) d
+                   ); 
+        [|destruct  ((C t a) / Delta) as [[ e d ]| ]; simpl; easy]. 
+        clear IHa H.
+        generalize (C t a) as T. intros T. clear a.
+        
+        induction T. destruct a as [[rA gA] eA]. 
+        simpl in *. 
+        case_eq (eval_expr Bool gA); intros H.  simpl.
+        unfold compose_block; simpl compose.  
+        induction (C u (f rA)). simpl. destruct a as [[rB gB] eB]. simpl. 
+        * rewrite eval_neffects_append. rewrite eval_andb_true. rewrite H. simpl. reflexivity. 
+        * simpl. rewrite H0. reflexivity.         
+
+        * unfold compose_block. simpl. induction (C u (f rA)). destruct a as [[rB gB] eB]. simpl. 
+          rewrite eval_andb_true. rewrite H. reflexivity.  
+          simpl. rewrite H0. reflexivity. 
+        * unfold compose_block. simpl. unfold compose_block in H. rewrite H. reflexivity.
+
+      - simpl. intros. 
+          Ltac t :=
+            repeat match goal with 
+                     | |- context [check ?x ; ?y] => 
+                         let H := fresh "check" in 
+                           case_eq x; intros H
+                   end. 
+          t; trivial. 
+      -                         (* primitive *)
+      intros. destruct p.  
+        +  simpl. reflexivity. 
+        + simpl.
+              
+          set (x := DList.to_tuple eval_expr exprs). 
+          replace (x) with (fst x, snd x) by (destruct x; reflexivity).
+
+          Lemma convert_commute  l (dl : DList.T (expr eval_type) l): map  _ _ _ (eval_expr) l (convert _ l dl) = DList.to_tuple (eval_expr) dl. 
+          Proof. 
+            induction dl. simpl. reflexivity. 
+            simpl. f_equal. apply IHdl. 
+          Qed. 
+          simpl. 
+    
+          replace (eval_expr t (fst (convert eval_type [t] exprs))) with (fst x). reflexivity. 
+          subst x. rewrite <- convert_commute. simpl. reflexivity.  
+
+        + simpl. 
+          rewrite <- convert_commute. simpl. reflexivity.
+        + simpl. 
+          rewrite <- convert_commute. simpl. 
+          case_eq (convert eval_type ([Tlift (Tfin n); t])%list exprs). 
+          intros adr [value tt] H.  simpl. simpl in tt.           
+          reflexivity. 
+
+      - intros. simpl.   unfold Sem.Dyn.OrElse. 
+        rewrite <- IHa1, <- IHa2 . clear IHa1 IHa2. 
+        generalize (C t a1); intros T; generalize (C t a2); intros T'. 
+        induction T as [[[rA gA] eA] |]; simpl.
+        induction T' as [[[rA' gA'] eA'] |]. simpl compose.
+        t. simpl. rewrite check0. simpl.  t. reflexivity. 
+        simpl. rewrite check0. simpl. t; reflexivity.  
+        simpl. unfold compose_block in *. simpl in *.  rewrite H. reflexivity. 
+        simpl. unfold compose_block in *. simpl in *.  rewrite H. reflexivity. 
+
+    Qed.
+    
+End correctness.     
+End t. 
+Notation "x <- e1 ; e2" := (@telescope_bind _ _ _ _ e1 (fun x => e2)) (right associativity, at level 80, e1 at next level).  
+Notation " & e " := (@telescope_end _ _ _ e) (at level 71). 
+Notation "e :- t1 ; t2 " := (@compose _ _ _ _ t1 (fun e => t2)) (right associativity, at level 80, t1 at next level).
+
+Notation Cs  := (compile_neffects _ _ ). 
+Notation C  := (compile_neffect _ _). 
+Notation Psi := (init_effects _ _). 
+
+Theorem nblock_compile_correct Phi (st : eval_state Phi) t (nb : nblock Phi eval_type t)  Delta:
+  eval_block Phi st _  (nblock_to_block Phi eval_type nb) Delta =  eval_nblock Phi st _ nb Delta. 
+unfold nblock in nb. 
+induction nb as [[[rA gA] eA]|]. unfold nblock_to_block. unfold compose_block. simpl.
+revert Delta t rA gA st . induction eA. simpl.
+intros. case_eq (eval_expr Bool gA); try reflexivity. intros. 
+f_equal. f_equal. 
+clear. 
+Lemma eval_effect_init Phi st Delta :   eval_effect Phi st (init_effects Phi eval_type) Delta = Delta. 
+Proof. 
+  induction Phi. reflexivity.
+destruct st as [hd tl].
+destruct Delta as [delta Delta].
+simpl.   
+f_equal.  apply IHPhi.  
+Qed. 
+now (apply eval_effect_init). 
+intros.  simpl eval_neffects. rewrite <- IHeA.  clear IHeA.
+simpl compile_neffects.
+
+Lemma foo {Phi R A B C} (T: telescope Phi R A) (f : A -> telescope Phi R B)  (g : B -> telescope Phi R C) : 
+  (X :- (Y :- T; f Y); (g X) )= (Y :- T; X :- f Y; g X). 
+Proof. 
+  induction T. reflexivity. simpl.
+  f_equal. 
+  Require Import  FunctionalExtensionality. 
+  apply functional_extensionality. 
+  apply H. 
+Qed. 
+rewrite foo.
+Lemma my_ind (Phi : state) (R : type -> Type) (P : neffect Phi R -> Prop) :
+  (forall (guard : expr R Bool) ,
+        P (neffect_guard Phi R guard [])) ->
+  (forall (guard : expr R Bool) a l ,
+        P a -> P (neffect_guard Phi R guard l) ->
+        P (neffect_guard Phi R guard (a :: l))) ->
+  (forall (t : type) (v : var Phi (Treg t)) (r : R t),
+     P (neffect_reg_write Phi R t v r)) ->
+  (forall (n : nat) (t : type) (v : var Phi (Tregfile n t))
+          (r : R (Tlift (Tfin n))) (r0 : R t),
+     P (neffect_regfile_write Phi R n t v r r0)) ->
+  forall n : neffect Phi R, P n. 
+Admitted. 
+Lemma correspondance Phi l : forall g1 g2, 
+  compile_neffect Phi eval_type g1 (neffect_guard Phi eval_type g2 l) Psi =
+  (compile_neffects Phi eval_type (g1 && g2)%expr l Psi).                  
+induction l. simpl. reflexivity. 
+simpl. 
+intros. reflexivity. 
+Qed. 
+Lemma eval_neffect_cons Phi st guard a l Delta: 
+  eval_neffect Phi st (neffect_guard Phi eval_type guard (a :: l)) Delta = 
+ (if eval_expr Bool guard
+  then eval_neffects Phi st l (eval_neffect Phi st a Delta)
+else Delta). reflexivity. 
+Qed. 
+
+Lemma eval_block_cons  Phi st t a : forall Delta guard f, 
+  eval_block Phi st t (X :- C guard a Psi; f X) Delta = 
+  eval_block Phi st t (f Psi) (if eval_expr _  guard then eval_neffect Phi st a Delta else Delta). 
+
+induction a using my_ind. 
+- intros. simpl. destruct (eval_expr Bool guard); destruct (eval_expr _ guard0); reflexivity. 
+- intros. rewrite correspondance. 
+intros. rewrite eval_neffect_cons. simpl.   
+rewrite foo.
+rewrite IHa. clear IHa. simpl. setoid_rewrite correspondance in IHa0.
+simpl compose in IHa0. simpl eval_block in IHa0 at 1. rewrite IHa0. clear IHa0. 
+case_eq (eval_expr Bool guard); intros; case_eq (eval_expr _ guard0); intros. 
+simpl Datatypes.andb. cbv iota. f_equal. admit. 
+simpl. reflexivity. 
+intros. unfold Datatypes.andb.
+f_equal. admit. 
+
+intros. simpl.  reflexivity. 
+- intros. simpl. unfold Diff.add. clear.
+unfold update_Treg. 
+case_eq (Tuple.get Phi (Treg t0) v Delta);
+case_eq (Tuple.get Phi (Treg t0) v (init_effects Phi eval_type)). intros. simpl. 
+ 
+unfold eval_block. 
+Admitted. 
+rewrite eval_block_cons. 
+simpl. reflexivity.  
+simpl. rewrite <- H. clear H. reflexivity. 
+Qed. 
+
+Print Assumptions nblock_compile_correct. 
+
+
+
+    
+End correctness. 
+
+  
+  Section defs2. 
+  Variable R : type -> Type. 
+  
   
   Arguments effect_guard guard%expr effects%list. 
   
@@ -87,10 +634,18 @@ Section t.
                 x <- (bind_expr _ exp); 
                 & (varunit, !x, nil)%expr
             | Primitive args res p exprs => _
-            | Try A => 
+            (* | Try A =>  *)
+            (*     [< rA, gA, eA >] :- compile _ A; *)
+            (*     let e := effect_guard gA eA in *)
+            (*       & (varunit, #b true, [e])%list *)
+            (*     (* & (varunit, gA, eA) *) *)
+            | OrElse t A A' => 
                 [< rA, gA, eA >] :- compile _ A;
+                [< rA', gA', eA' >] :- compile _ A';
                 let e := effect_guard gA eA in 
-                  & (varunit, #b true, [e])%list
+                let e' := effect_guard ((~ gA) &&  gA')%expr eA' in 
+                  r <- (bind_expr _ (Emux _ _ gA (!rA) (!rA'))%expr); 
+                  & ( r , (gA || gA')%expr , [e;e'])%list
           end in f t a).
   (* primitive *)
   revert exprs. 
@@ -126,6 +681,8 @@ Section t.
                      &( varunit, #b true, e)                      
              end
          ). 
+    (* or else *)
+  
   Defined. 
   
   Definition wrap t (T : preblock t) : block. 
@@ -151,22 +708,25 @@ Section t.
            ). 
     Defined. 
     
-  
-    Fixpoint eval_effect (e :effect eval_type) (Delta : updates) : option updates :=    
+    Definition up {A} (x : option A) y := match x with None => y | Some y => y end.  
+                                                                
+    Fixpoint eval_effect (e :effect eval_type) (Delta : updates) : updates :=    
       match e with 
-      | effect_guard g l' => 
-          let fix eval_effects l Delta := 
-              match l with 
-                | nil => Some Delta
-                | cons e q =>  do Delta <- eval_effect e Delta; 
-                    eval_effects q Delta
-              end in     
-            match eval_expr _ g with 
-              | true =>  match eval_effects l' Delta with
-                            | Some Delta => Some Delta
-                            | None => Some Delta
-                        end
-              | false => Some Delta
+        | effect_guard g l' => 
+            let fix eval_effects l Delta := 
+                match l with 
+                  | nil => Delta
+                  | cons e q =>  
+                      let Delta := eval_effect e Delta in 
+                        eval_effects q Delta
+                end in     
+              match eval_expr _ g with 
+                | true =>  (* match eval_effects l' Delta with *)
+                    (*     | Some Delta => Some Delta *)
+                    (*     | None => Some Delta *)
+                        (* end                         *)
+                    eval_effects l' Delta
+                | false => Delta
             end
       | effect_reg_write t v w =>                                               
           Core.Diff.add Phi Delta (Treg t) v w 
@@ -176,24 +736,41 @@ Section t.
               Core.Diff.add Phi Delta (Tregfile n t) v rf            
     end. 
   
-    Fixpoint eval_effects ( l : list (effect eval_type)) Delta : option updates :=
+    Fixpoint eval_effects ( l : list (effect eval_type)) Delta : updates :=
       match l with 
-        | nil => Some Delta
-        | cons e q => do Delta <- eval_effect e Delta; 
+        | nil =>  Delta
+        | cons e q => (* do Delta <- eval_effect e Delta;  *)
+            let Delta :=  (eval_effect e Delta) in 
             eval_effects q Delta
       end. 
   
     Lemma fold_eval_effects :
       (fix eval_effects l Delta := 
        match l with 
-                | nil => Some Delta
-                | cons e q =>  do Delta <- eval_effect e Delta; 
-                    eval_effects q Delta
+                | nil =>  Delta
+                | cons e q => 
+                    let Delta := (eval_effect e Delta) in 
+                      (* do Delta <- eval_effect e Delta;  *)
+                      eval_effects q Delta
        end)= eval_effects .
     Proof. 
       unfold eval_effects. reflexivity.
     Qed. 
     
+    (* Lemma eval_effects_cons  t q Delta :  *)
+    (*   eval_effects (t :: q) Delta = do Delta' <- eval_effect  t Delta; eval_effects q Delta'.  *)
+    (* Proof. *)
+    (*   reflexivity.  *)
+    (* Qed.  *)
+    
+    (* Lemma eval_effect_guard (gA : expr eval_type Bool) eA Delta:  *)
+    (*   eval_expr  _ gA = true -> *)
+    (*   eval_effect  (effect_guard eval_type gA eA) Delta = eval_effects eA Delta.  *)
+    (* Proof.  *)
+    (*   intros. simpl. rewrite (fold_eval_effects).  *)
+    (*   rewrite H. reflexivity.  *)
+    (* Qed.  *)
+
     Fixpoint eval_preblock t  (T : preblock  eval_type t) :
       updates -> option (eval_type t * updates) := 
       match T with
@@ -203,21 +780,19 @@ Section t.
               eval_preblock _ (cont res) Delta
         | telescope_end (p, g, e) => fun Delta =>
                                       let g := eval_expr _ g  in             
-                                      if g then 
-                                        do x <- eval_effects e Delta;
-                                        Some (p, x)
+                                      if g then                                         
+                                        Some (p, eval_effects e Delta)
                                       else None
     end. 
   
   
-    Fixpoint eval_block (a : block eval_type) {struct a}: updates -> option updates :=
+    Fixpoint eval_block (a : block eval_type) {struct a}: updates ->  updates :=
       match a with
         | telescope_bind arg bind cont => 
             fun Delta => 
               let res  := eval_bind _ bind in 
                 eval_block (cont res) Delta
-        | telescope_end effects => 
-            eval_effects effects
+        | telescope_end effects => eval_effects effects
       end. 
     
   End sem. 
@@ -240,15 +815,15 @@ Section t.
 
     Lemma eval_effects_append  st e f (Delta : updates) : 
       eval_effects st (e ++ f) Delta = 
-                   do D <- eval_effects st e Delta; eval_effects st f D.              
+                   eval_effects st f (eval_effects st e Delta).              
     Proof. 
       revert Delta. 
       induction e. 
       + reflexivity. 
       + intros Delta.
         
-        simpl. case_eq (eval_effect st a Delta). intros. apply IHe. 
-        reflexivity. 
+        simpl. rewrite IHe. reflexivity.  
+
     Qed. 
 
     Variable st : eval_state Phi. 
@@ -271,94 +846,60 @@ Section t.
         
         induction T. destruct a as [[rA gA] eA]. 
         simpl in *. 
-        case_eq (eval_expr Bool gA); intros H.  
-        case_eq (eval_effects st eA Delta). 
-        + intros D HD.
-          unfold Common.bind. 
-          generalize (C u (f rA)).  intros T'. clear rA. 
-          induction T'. destruct a as [[rB gB] eB]. simpl. 
-          rewrite eval_andb_true. rewrite H. simpl. 
+        case_eq (eval_expr Bool gA); intros H.  simpl.
+        induction (C u (f rA)). destruct a as [[rB gB] eB]. simpl. 
+        * rewrite eval_effects_append. rewrite eval_andb_true. rewrite H. simpl. reflexivity. 
+        * simpl. rewrite H0. reflexivity.         
+
+        * induction (C u (f rA)). destruct a as [[rB gB] eB]. simpl. 
+          rewrite eval_andb_true. rewrite H. reflexivity.  
+          simpl. rewrite H0. reflexivity. 
+        * simpl. rewrite H. reflexivity.
+
+      - simpl. intros. 
           Ltac t :=
             repeat match goal with 
                      | |- context [check ?x ; ?y] => 
                          let H := fresh "check" in 
                            case_eq x; intros H
                    end. 
-          t; trivial.   
-          rewrite eval_effects_append. rewrite HD. reflexivity. 
-          simpl. 
-          rewrite <- H0. reflexivity. 
-        + intros HD.
-          unfold Common.bind. 
-          generalize (C u (f rA)).  intros T'. 
-          induction T'. destruct a as [[rB gB] eB]. simpl. 
-          rewrite eval_andb_true. rewrite H. simpl. 
-          t; try reflexivity. 
-          rewrite eval_effects_append. rewrite HD. reflexivity. 
-          
-          simpl. 
-          apply H0. 
-          
-        +  unfold Common.bind. generalize (C u (f rA)).  intros T'. 
-          induction T'. destruct a as [[rB gB] eB]. simpl. 
-          rewrite eval_andb_true. rewrite H. simpl. reflexivity. 
-          
-          simpl. unfold Common.bind.  
-          apply H0. 
-
-        + simpl. unfold Common.bind.  
-          simpl. apply H. 
-
-      - intros. 
-        simpl. 
-        t. reflexivity.  reflexivity. 
-
-      - intros. 
-        simpl. destruct p.
+          t; trivial. 
+      -                         (* primitive *)
+      intros. destruct p.  
         +  simpl. reflexivity. 
-        + simpl. 
-          unfold Common.bind.
+        + simpl.
+              
           set (x := DList.to_tuple eval_expr exprs). 
           replace (x) with (fst x, snd x) by (destruct x; reflexivity).
+
           Lemma convert_commute  l (dl : DList.T (expr eval_type) l): map  _ _ _ (eval_expr) l (convert _ l dl) = DList.to_tuple (eval_expr) dl. 
           Proof. 
             induction dl. simpl. reflexivity. 
             simpl. f_equal. apply IHdl. 
           Qed. 
-            
+          simpl. 
     
-          replace (eval_expr t (fst (convert eval_type [t] exprs))) with (fst x). 
-          case_eq (Diff.add Phi Delta (Treg t) v (fst x)); trivial.
-          subst x. rewrite <- convert_commute. simpl. reflexivity. 
+          replace (eval_expr t (fst (convert eval_type [t] exprs))) with (fst x). reflexivity. 
+          subst x. rewrite <- convert_commute. simpl. reflexivity.  
+
         + simpl. 
           rewrite <- convert_commute. simpl. reflexivity.
         + simpl. 
           rewrite <- convert_commute. simpl. 
           case_eq (convert eval_type ([Tlift (W p); t])%list exprs). 
-          intros adr [value tt] H.  simpl. simpl in tt. 
-          case_eq ( Diff.add Phi Delta (Tregfile n t) v
-       (Regfile.set (Tuple.get Phi (Tregfile n t) v st)
-          (Word.unsigned (eval_expr (Tlift (W p)) adr)) 
-          (eval_expr t value))). 
-          intros. 
-          simpl. reflexivity. 
-          intros. simpl. reflexivity. 
+          intros adr [value tt] H.  simpl. simpl in tt.           
+          reflexivity. 
 
-      - intros.
-        simpl. unfold Sem.Dyn.Try. rewrite <- IHa; clear IHa.
-        generalize (C Unit a). intros T. induction T. 
+      - intros. simpl.   unfold Sem.Dyn.OrElse. 
+        rewrite <- IHa1, <- IHa2 . clear IHa1 IHa2. 
+        generalize (C t a1); intros T; generalize (C t a2); intros T'. 
+        induction T as [[[rA gA] eA] |]; simpl.
+        induction T' as [[[rA' gA'] eA'] |]. simpl compose.
+        t. simpl. rewrite check0. simpl.  t. reflexivity. 
+        simpl. rewrite check0. simpl. t; reflexivity.  
+        simpl. rewrite H. reflexivity. 
+        simpl. rewrite H. reflexivity.
 
-        * destruct a0 as [[rA gA] eA]. 
-        simpl compose. 
-        simpl; rewrite (fold_eval_effects st).
-        t. 
-        destruct (eval_effects st eA Delta); simpl; [destruct rA; reflexivity|].  reflexivity. 
-
-        simpl.  reflexivity. 
-
-        * simpl. 
-          rewrite H.  reflexivity. 
-          
     Qed.
 End correctness. 
 End t. 
